pulse/lib/pulse/lib/Pulse.Lib.CancellableInvariant.fsti
@@ -28,9 +28,9 @@ val cinv_vp (c:cinv) (v:slprop) : slprop
 
 val active (c:cinv) (p:perm) : slprop
 
-val active_is_slprop2 (c:cinv) (p:perm)
-  : Lemma (is_slprop2 (active c p))
-          [SMTPat (is_slprop2 (active c p))]
+val active_timeless (c:cinv) (p:perm)
+  : Lemma (timeless (active c p))
+          [SMTPat (timeless (active c p))]
 
 val iname_of (c:cinv) : GTot iname
 
