pulse/lib/pulse/lib/Pulse.Lib.Codeable.fsti
@@ -7,7 +7,7 @@ as "big" slprops (i.e. slprop3). *)
 noeq
 type vcode : Type u#4 = {
     t : Type u#2;
-    up : t -> slprop3;
+    up : t -> slprop;
 }
 
 (* A class for codeable slprops. *)
@@ -21,18 +21,3 @@ let encode (#code:vcode) (v:slprop) {| d : codeable code v |} : code.t =
 
 let decode (#code:vcode) (c:code.t) : slprop =
   code.up c
-
-(* Small slprops (slprop2) form a trivial code by lifting with up3. *)
-let small_code : vcode = {
-  t = slprop2_base;
-  up = (fun c -> up2_is_slprop2 c; Pulse.Lib.Core.up2 c);
-}
-
-(* A codeable instance for small slprops. Note: this only triggers if
-there is an instance for Pulse.Class.Small.small for the given slprop (instead of
-requiring (squash (is_slprop2 v)), since typeclass instantiation cannot backtrack if
-a refinement proof fails. *)
-instance codeable_small (v:slprop) (_ : Pulse.Class.Small.small v) : codeable small_code v = {
-  code_of = down2 v;
-  pf = ();
-}
